securedrop-protocol/protocol-minimal/proofs/fstar/models/Libcrux_chacha20poly1305.Hacl.Aead_chacha20poly1305.fsti
@@ -31,3 +31,63 @@ val encrypt
       (data_len: u32)
       (key nonce: t_Slice u8)
     : Prims.Pure (t_Slice u8 & t_Slice u8) Prims.l_True (fun _ -> Prims.l_True)
+
+let decrypt__i: u32 = mk_u32 0 +! (mk_u32 0 *! mk_u32 1 <: u32)
+
+let decrypt__ii_1: u32 = mk_u32 0 +! (mk_u32 1 *! mk_u32 1 <: u32)
+
+let decrypt__ii_2: u32 = mk_u32 0 +! (mk_u32 2 *! mk_u32 1 <: u32)
+
+let decrypt__ii_3: u32 = mk_u32 0 +! (mk_u32 3 *! mk_u32 1 <: u32)
+
+let decrypt__ii_4: u32 = mk_u32 0 +! (mk_u32 4 *! mk_u32 1 <: u32)
+
+let decrypt__ii_5: u32 = mk_u32 0 +! (mk_u32 5 *! mk_u32 1 <: u32)
+
+let decrypt__ii_6: u32 = mk_u32 0 +! (mk_u32 6 *! mk_u32 1 <: u32)
+
+let decrypt__ii_7: u32 = mk_u32 0 +! (mk_u32 7 *! mk_u32 1 <: u32)
+
+let decrypt__ii_8: u32 = mk_u32 0 +! (mk_u32 8 *! mk_u32 1 <: u32)
+
+let decrypt__ii_9: u32 = mk_u32 0 +! (mk_u32 9 *! mk_u32 1 <: u32)
+
+let decrypt__ii_10: u32 = mk_u32 0 +! (mk_u32 10 *! mk_u32 1 <: u32)
+
+let decrypt__ii_11: u32 = mk_u32 0 +! (mk_u32 11 *! mk_u32 1 <: u32)
+
+let decrypt__ii_12: u32 = mk_u32 0 +! (mk_u32 12 *! mk_u32 1 <: u32)
+
+let decrypt__ii_13: u32 = mk_u32 0 +! (mk_u32 13 *! mk_u32 1 <: u32)
+
+let decrypt__ii_14: u32 = mk_u32 0 +! (mk_u32 14 *! mk_u32 1 <: u32)
+
+let decrypt__ii_15: u32 = mk_u32 0 +! (mk_u32 15 *! mk_u32 1 <: u32)
+
+(**
+Decrypt a ciphertext `input` with key `key`.
+
+The arguments `key`, `nonce`, `data`, and `data_len` are same in encryption/decryption.
+Note: Encryption and decryption can be executed in-place, i.e., `output` and `input` can point to the same memory.
+
+If decryption succeeds, the resulting plaintext is stored in `output` and the function returns the success code 0.
+If decryption fails, the array `output` remains unchanged and the function returns the error code 1.
+
+@param output Pointer to `input_len` bytes of memory where the message is written to.
+@param input Pointer to `input_len` bytes of memory where the ciphertext is read from.
+@param input_len Length of the ciphertext.
+@param data Pointer to `data_len` bytes of memory where the associated data is read from.
+@param data_len Length of the associated data.
+@param key Pointer to 32 bytes of memory where the AEAD key is read from.
+@param nonce Pointer to 12 bytes of memory where the AEAD nonce is read from.
+@param tag Pointer to 16 bytes of memory where the mac is read from.
+
+@returns 0 on succeess; 1 on failure.
+*)
+val decrypt
+      (output input: t_Slice u8)
+      (input_len: u32)
+      (data: t_Slice u8)
+      (data_len: u32)
+      (key nonce tag: t_Slice u8)
+    : Prims.Pure (t_Slice u8 & u32) Prims.l_True (fun _ -> Prims.l_True)
