securedrop-protocol/protocol-minimal/proofs/fstar/models/Libcrux_chacha20poly1305.Impl_hacl.fsti
@@ -3,6 +3,14 @@ module Libcrux_chacha20poly1305.Impl_hacl
 open FStar.Mul
 open Core_models
 
+let v_NOT_DETACHED: bool = false
+
+val encrypt_checks (ptxt ctxt aad: t_Slice u8) (detached: bool)
+    : Prims.Pure
+      (t_Slice u8 & Core_models.Result.t_Result (u32 & u32) Libcrux_chacha20poly1305.t_AeadError)
+      Prims.l_True
+      (fun _ -> Prims.l_True)
+
 /// The ChaCha20-Poly1305 AEAD encryption function. Writes the concatenation of the ciphertext
 /// produced by ChaCha20 and the MAC tag into `ctxt` and returns the two pieces separately.
 /// This implementation is backed by hacl-rs and can only handle inputs up to a length of `u32::MAX`.
@@ -12,8 +20,7 @@ val encrypt
       (ptxt ctxt aad: t_Slice u8)
       (nonce: t_Array u8 (mk_usize 12))
     : Prims.Pure
-      (t_Slice u8 &
-        Core_models.Result.t_Result (t_Slice u8 & t_Array u8 (mk_usize 16))
+      (Core_models.Result.t_Result (t_Slice u8 & t_Array u8 (mk_usize 16))
           Libcrux_chacha20poly1305.t_AeadError) Prims.l_True (fun _ -> Prims.l_True)
 
 /// The ChaCha20-Poly1305 AEAD decryption function. Writes the result of the decryption to `ptxt`,
